src/Eval.v
@@ -10,9 +10,14 @@ Require Import
 From Equations Require Import Equations.
 Set Equations With UIP.
 
+Section Eval.
+
 Generalizable All Variables.
 
 Import ListNotations.
+
+Context {A : Type}.
+Context `{S : HostExprsSem A}.
 
 Reserved Notation " t '--->' t' " (at level 40).
 
@@ -24,6 +29,8 @@ Inductive Step : ∀ {Γ τ}, Exp Γ τ → Exp Γ τ → Prop :=
   | ST_Seq Γ τ τ' (e1 : Exp Γ τ') (e2 : Exp Γ τ) :
     Seq e1 e2 ---> e2
 
+  | ST_IfHost Γ (b : HostExp TyBool) τ (t e : Exp Γ τ) :
+    If (Hosted b) t e ---> If (GetBool b) t e
   | ST_IfTrue Γ τ (t e : Exp Γ τ) :
     If ETrue t e ---> t
   | ST_IfFalse Γ τ (t e : Exp Γ τ) :
@@ -39,6 +46,9 @@ Inductive Step : ∀ {Γ τ}, Exp Γ τ → Exp Γ τ → Prop :=
     ValueP x →
     y ---> y' →
     Pair x y ---> Pair x y'
+
+  | ST_FstHost Γ τ1 τ2 (p : HostExp (TyPair τ1 τ2)) :
+    Fst (Hosted p) ---> Fst (GetPair (Γ:=Γ) p)
   | ST_Fst1 Γ τ1 τ2 (p p' : Exp Γ (TyPair τ1 τ2)) :
     p ---> p' →
     Fst p ---> Fst p'
@@ -46,6 +56,9 @@ Inductive Step : ∀ {Γ τ}, Exp Γ τ → Exp Γ τ → Prop :=
     ValueP v1 →
     ValueP v2 →
     Fst (Pair v1 v2) ---> v1
+
+  | ST_SndHost Γ τ1 τ2 (p : HostExp (TyPair τ1 τ2)) :
+    Snd (Hosted p) ---> Snd (GetPair (Γ:=Γ) p)
   | ST_Snd1 Γ τ1 τ2 (p p' : Exp Γ (TyPair τ1 τ2)) :
     p ---> p' →
     Snd p ---> Snd p'
@@ -53,6 +66,10 @@ Inductive Step : ∀ {Γ τ}, Exp Γ τ → Exp Γ τ → Prop :=
     ValueP v1 →
     ValueP v2 →
     Snd (Pair v1 v2) ---> v2
+
+  | ST_AppHost Γ dom cod (f : HostExp (dom ⟶ cod)) (v : Exp Γ dom) :
+    ∀ H : ValueP v,
+    APP (Hosted f) v ---> CallHost f v H
 
   | ST_AppAbs Γ dom cod (e : Exp (dom :: Γ) cod) (v : Exp Γ dom) :
     ValueP v →
@@ -71,26 +88,79 @@ Inductive Step : ∀ {Γ τ}, Exp Γ τ → Exp Γ τ → Prop :=
 
 Derive Signature for Step.
 
-Ltac reduce :=
-  repeat (lazymatch goal with
-          | [ H : existT _ _ _ = existT _ _ _ |- _ ] =>
-              apply inj_pair2 in H; subst
-          | [ H : _ ∧ _ |- _ ] => destruct H
-          | [ H : _ * _ |- _ ] => destruct H
-          | [ H : ∃ _, _ |- _ ] => destruct H
-          end; subst).
+End Eval.
 
-Ltac inv H := inversion H; subst; clear H; reduce.
+Notation " t '--->' t' " := (Step t t') (at level 40).
+
+Class HostLang (A : Type) : Type := {
+  has_host_exprs_sem :> HostExprsSem A;
+
+
+  CallHost_sound {Γ dom cod} (f : HostExp (dom ⟶ cod))
+                 (v : Exp Γ dom) (H : ValueP v) se :
+    HostExpSem f (SemExp v se) = SemExp (CallHost f v H) se;
+
+  CallHost_irr {Γ dom cod} (f : HostExp (dom ⟶ cod))
+               (v : Exp Γ dom) (H : ValueP v) :
+    ¬ (CallHost f v H = APP (Hosted f) v);
+
+  CallHost_preserves_renaming {Γ Γ' dom cod} (f : HostExp (dom ⟶ cod))
+               (v : Exp Γ dom) (H : ValueP v) (σ : Ren Γ' Γ) :
+    APP (Hosted f) (RenExp σ v) ---> RenExp σ (CallHost f v H);
+
+  CallHost_preserves_substitution {Γ Γ' dom cod} (f : HostExp (dom ⟶ cod))
+               (v : Exp Γ dom) (H : ValueP v) (σ : Sub Γ' Γ) :
+    APP (Hosted f) (SubExp σ v) ---> SubExp σ (CallHost f v H);
+
+
+  GetBool_sound {Γ} (b : HostExp TyBool) se :
+    HostExpSem b = SemExp (GetBool (Γ:=Γ) b) se;
+
+  GetBool_irr {Γ} (b : HostExp TyBool) :
+    ¬ (Hosted b = GetBool (Γ:=Γ) b);
+
+  GetBool_preserves_renaming {Γ Γ'} (b : HostExp TyBool) (σ : Ren Γ Γ') :
+    RenExp σ (Hosted b) ---> RenExp σ (GetBool b);
+
+  GetBool_preserves_substitution {Γ Γ'} (b : HostExp TyBool) (σ : Sub Γ Γ') :
+    SubExp σ (Hosted b) ---> SubExp σ (GetBool b);
+
+
+  GetPair_sound {Γ τ1 τ2} (p : HostExp (TyPair τ1 τ2)) se :
+    HostExpSem p = SemExp (GetPair (Γ:=Γ) p) se;
+
+  GetPair_irr {Γ τ1 τ2} (p : HostExp (TyPair τ1 τ2)) :
+    ¬ (Hosted p = GetPair (Γ:=Γ) p);
+
+  GetPair_preserves_renaming {Γ Γ' τ1 τ2} (p : HostExp (TyPair τ1 τ2))
+                             (σ : Ren Γ Γ') :
+    RenExp σ (Hosted p) ---> RenExp σ (GetPair p);
+
+  GetPair_preserves_substitution {Γ Γ' τ1 τ2} (p : HostExp (TyPair τ1 τ2))
+                                 (σ : Sub Γ Γ') :
+    SubExp σ (Hosted p) ---> SubExp σ (GetPair p);
+}.
+
+Section Sound.
+
+Context {A : Type}.
+Context `{L : HostLang A}.
 
 Theorem Step_sound {Γ τ} (e : Exp Γ τ) v :
   e ---> v → SemExp e = SemExp v.
 Proof.
   intros.
-  induction H; simpl; auto;
-  extensionality E;
+  dependent induction H; simpl; auto;
+  extensionality se;
   try now rewrite IHStep.
+  - now erewrite GetBool_sound; eauto.
+  - now erewrite GetPair_sound; eauto.
+  - now erewrite GetPair_sound; eauto.
+  - now apply CallHost_sound.
   - rewrite <- SemExp_SubSem.
     f_equal; simpl.
     simp SubSem.
     now rewrite SubSem_idSub.
 Qed.
+
+End Sound.
