src/Lit.v
@@ -16,3 +16,20 @@ Inductive Literal : PrimType → Set :=
   | LTime    : UTCTime → Literal PrimTime.
 
 Derive NoConfusion for Literal.
+
+Definition SemPrim (p : PrimType) : Type :=
+  match p with
+  | PrimInteger => Z
+  | PrimDecimal => Q
+  | PrimTime    => UTCTime
+  | PrimString  => string
+  end.
+
+Definition SemLit `(l : Literal ty) : SemPrim ty :=
+  match l with
+  | LString  s => s
+  | LInteger z => z
+  | LDecimal q => q
+  | LTime    t => t
+  end.
+
