src/Ty.v
@@ -4,13 +4,15 @@ Require Export
 From Equations Require Import Equations.
 Set Equations With UIP.
 
-Inductive PrimType : Type :=
-  | PrimInteger
-  | PrimDecimal
-  | PrimTime
-  | PrimString.
+Section Ty.
 
-Derive NoConfusion for PrimType.
+Class HostTypes (A : Type) : Type := {
+  HostTy : Type;
+  HostTySem : HostTy → Type
+}.
+
+Context {A : Type}.
+Context `{HostTypes A}.
 
 (* TODO:
  - Lists
@@ -23,7 +25,7 @@ Derive NoConfusion for PrimType.
  - Capabilities *)
 
 Inductive Ty : Type :=
-  | TyPrim : PrimType → Ty
+  | TyHost : HostTy → Ty
 
   | TyUnit : Ty
   | TyBool : Ty
@@ -34,15 +36,18 @@ Inductive Ty : Type :=
 
 Derive NoConfusion Subterm for Ty.
 
+End Ty.
+
+Arguments Ty {A H}.
+Arguments TyHost {A H} _.
+Arguments TyUnit {A H}.
+Arguments TyBool {A H}.
+Arguments TyPair {A H} _ _.
+Arguments TyArrow {A H} _ _.
+
 Declare Scope Ty_scope.
 Bind Scope Ty_scope with Ty.
 Delimit Scope Ty_scope with ty.
 
 Infix "⟶" := TyArrow (at level 30, right associativity) : Ty_scope.
 Infix "×"  := TyPair  (at level 40, left associativity) : Ty_scope.
-
-Definition ℤ := TyPrim PrimInteger.
-Definition ℝ := TyPrim PrimDecimal.
-Definition 𝕋 := TyPrim PrimTime.
-Definition 𝕊 := TyPrim PrimString.
-Definition 𝔹 := TyBool.
