src/Unit.v
@@ -1,0 +1,32 @@
+Require Export
+  Ty
+  Exp
+  Sem.
+
+Inductive UnitT := TyUnit.
+
+Derive NoConfusion for UnitT.
+
+Definition Unit_HostTypes : HostTypes unit := {|
+  HostTy := UnitT;
+  HostTySem := λ 'UnitT, unit
+|}.
+
+Inductive UnitE : Ty → Type :=
+  | EUnit : UnitE (@TyHost _ Unit_HostTypes TyUnit).
+
+Derive NoConfusion for UnitE.
+
+Definition Unit_HostExprs : HostExprs unit := {|
+  has_host_types := Unit_HostTypes;
+  HostExp := UnitE
+|}.
+
+Equations Unit_HostExpSem τ (e : HostExp (HostExprs:=Unit_HostExprs) τ) :
+  SemTy τ := Unit_HostExpSem (TyHost TyUnit) EUnit := tt.
+
+Program Definition Unit_HostLang : HostLang unit := {|
+  has_host_exprs := Unit_HostExprs;
+  HostExpSem := Unit_HostExpSem
+|}.
+
